code/chacha20/Hacl.Spec.Chacha20.Lemmas.fst
@@ -5,37 +5,46 @@ open Lib.IntTypes
 open Lib.Sequence
 open Lib.IntVector
 open Lib.IntVector.Transpose
+open Lib.NTuple
 
 open Hacl.Spec.Chacha20.Vec
 
-#set-options "--z3rlimit 50 --max_fuel 0 --max_ifuel 0"
+#set-options "--z3rlimit 50 --fuel 0 --ifuel 0"
+
 
 /// (vec_v (transpose #w k).[i / w]).[i % w] == ((transpose_state k).[i / 16]).[i % 16]
 
 val transpose4_lemma: k:state 4 -> i:nat{i < 16 * 4} ->
   Lemma ((vec_v (transpose4 k).[i / 4]).[i % 4] == ((transpose_state k).[i / 16]).[i % 16])
 let transpose4_lemma st i =
-  // let (r0,(r1,(r2,r3))) = transposewxw #U32 #4 (st.[0],(st.[1],(st.[2],st.[3]))) in
-  // transposewxw_lemma #U32 #4 (st.[0],(st.[1],(st.[2],st.[3])));
-  // let (r4,(r5,(r6,r7))) = transposewxw #U32 #4 (st.[4],(st.[5],(st.[6],st.[7]))) in
-  // transposewxw_lemma #U32 #4 (st.[4],(st.[5],(st.[6],st.[7])));
-  // let (r8,(r9,(r10,r11))) = transposewxw #U32 #4 (st.[8],(st.[9],(st.[10],st.[11]))) in
-  // transposewxw_lemma #U32 #4 (st.[8],(st.[9],(st.[10],st.[11])));
-  // let (r12,(r13,(r14,r15))) = transposewxw #U32 #4 (st.[12],(st.[13],(st.[14],st.[15]))) in
-  // transposewxw_lemma #U32 #4 (st.[12],(st.[13],(st.[14],st.[15])));
-  admit()
+  let st0 : ntuple (vec_t U32 4) 4 = ntup4 (st.[0],(st.[1],(st.[2],st.[3]))) in
+  let (v0,(v1,(v2,v3))) = tup4 (transpose4x4 #U32 st0) in
+  transpose4x4_lemma #U32 st0;
+
+  let st1 : ntuple (vec_t U32 4) 4 = ntup4 (st.[4],(st.[5],(st.[6],st.[7]))) in
+  let (v4,(v5,(v6,v7))) = tup4 (transpose4x4 #U32 st1) in
+  transpose4x4_lemma #U32 st1;
+
+  let st2 : ntuple (vec_t U32 4) 4 = ntup4 (st.[8],(st.[9],(st.[10],st.[11]))) in
+  let (v8,(v9,(v10,v11))) = tup4 (transpose4x4 #U32 st2) in
+  transpose4x4_lemma #U32 st2;
+
+  let st3 : ntuple (vec_t U32 4) 4 = ntup4 (st.[12],(st.[13],(st.[14],st.[15]))) in
+  let (v12,(v13,(v14,v15))) = tup4 (transpose4x4 #U32 st3) in
+  transpose4x4_lemma #U32 st3
 
 
 val transpose8_lemma: k:state 8 -> i:nat{i < 16 * 8} ->
   Lemma ((vec_v (transpose8 k).[i / 8]).[i % 8] == ((transpose_state k).[i / 16]).[i % 16])
 let transpose8_lemma st i =
-  // let (v0,(v1,(v2,(v3,(v4,(v5,(v6,v7))))))) =
-  //   transposewxw #U32 #8 (st.[0],(st.[1],(st.[2],(st.[3],(st.[4],(st.[5],(st.[6],st.[7]))))))) in
-  // let (v8,(v9,(v10,(v11,(v12,(v13,(v14,v15))))))) =
-  //   transposewxw #U32 #8 (st.[8],(st.[9],(st.[10],(st.[11],(st.[12],(st.[13],(st.[14],st.[15]))))))) in
-  // transposewxw_lemma #U32 #8 (st.[0],(st.[1],(st.[2],(st.[3],(st.[4],(st.[5],(st.[6],st.[7])))))));
-  // transposewxw_lemma #U32 #8 (st.[8],(st.[9],(st.[10],(st.[11],(st.[12],(st.[13],(st.[14],st.[15])))))));
-  admit()
+  let st0 : ntuple (vec_t U32 8) 8 = ntup8 (st.[0],(st.[1],(st.[2],(st.[3],(st.[4],(st.[5],(st.[6],st.[7]))))))) in
+  let (v0,(v1,(v2,(v3,(v4,(v5,(v6,v7))))))) = tup8 (transpose8x8 #U32 st0) in
+
+  let st1 : ntuple (vec_t U32 8) 8 = ntup8 (st.[8],(st.[9],(st.[10],(st.[11],(st.[12],(st.[13],(st.[14],st.[15]))))))) in
+  let (v8,(v9,(v10,(v11,(v12,(v13,(v14,v15))))))) = tup8 (transpose8x8 #U32 st1) in
+  transpose8x8_lemma #U32 st0;
+  transpose8x8_lemma #U32 st1
+
 
 val transpose_lemma_index: #w:lanes -> k:state w -> i:nat{i < 16 * w} ->
   Lemma ((vec_v (transpose #w k).[i / w]).[i % w] == ((transpose_state k).[i / 16]).[i % 16])
